Weidenbach_Book/IsaSAT_Watch_List.thy
@@ -18,13 +18,6 @@ text \<open>There is not much to say about watch list,s since they are arrays of
   for eq.atree.braun.7.unsat.cnf instead of 7s).
 \<close>
 
-(* TODO Move *)
-instance uint64 :: semiring_numeral
-  by standard
-
-instance uint32 :: semiring_numeral
-  by standard
-(* End Move *)
 type_synonym watched_wl = \<open>((nat \<times> uint64) array_list) array\<close>
 type_synonym watched_wl_uint32 = \<open>((uint64 \<times> uint64) array_list) array\<close>
 
@@ -34,95 +27,6 @@ definition watcher_enc where
 
 definition take_only_lower32 :: \<open>uint64 \<Rightarrow> uint64\<close> where
   [code del]: \<open>take_only_lower32 n = n AND ((1 << 32) - 1)\<close>
-
-lemma bintrunc_eq_bits_eqI: \<open> (\<And>n. (n < r \<and> bin_nth c n) = (n < r \<and> bin_nth a n)) \<Longrightarrow>
-       bintrunc r (a) = bintrunc r c\<close>
-proof (induction r arbitrary: a c)
-  case 0
-  then show ?case by (simp_all flip: bin_nth.Z)
-next
-  case (Suc r a c) note IH = this(1) and eq = this(2)
-  have 1: \<open>(n < r \<and> bin_nth (bin_rest a) n) = (n < r \<and> bin_nth (bin_rest c) n)\<close> for n
-    using eq[of \<open>Suc n\<close>] eq[of 1] by (clarsimp simp flip: bin_nth.Z)
-  show ?case
-    using IH[OF 1] eq[of 0] by (simp_all flip: bin_nth.Z)
-qed
-
-lemma and_eq_bits_eqI: \<open>(\<And>n. c !! n = (a !! n \<and> b !! n))\<Longrightarrow> a AND b = c\<close> for a b c :: \<open>_ word\<close>
-  by transfer
-    (rule bintrunc_eq_bits_eqI, auto simp add: bin_nth_ops)
-
-
-lemma pow2_mono_word_less:
-   \<open>m < LENGTH('a) \<Longrightarrow> n < LENGTH('a) \<Longrightarrow> m < n \<Longrightarrow> (2 :: 'a :: len word) ^m  < 2 ^ n\<close>
-proof (induction n arbitrary: m)
-  case 0
-  then show ?case by auto
-next
-  case (Suc n m) note IH = this(1) and le = this(2-)
-  have [simp]: \<open>nat (bintrunc LENGTH('a) (2::int)) = 2\<close>
-    by (metis add_lessD1 le(2) plus_1_eq_Suc power_one_right uint_bintrunc unat_def unat_p2)
-  have 1: \<open>unat ((2 :: 'a word) ^ n) \<le> (2 :: nat) ^ n\<close>
-    by (metis Suc.prems(2) eq_imp_le le_SucI linorder_not_less unat_p2)
-  have 2: \<open>unat ((2 :: 'a word)) \<le> (2 :: nat)\<close>
-     by (metis le_unat_uoi nat_le_linear of_nat_numeral)
-  have \<open>unat (2 :: 'a word) * unat ((2 :: 'a word) ^ n) \<le> (2 :: nat) ^ Suc n\<close>
-    using mult_le_mono[OF 2 1] by auto
-  also have \<open>(2 :: nat) ^ Suc n < (2 :: nat) ^ LENGTH('a)\<close>
-    using le(2) by (metis unat_lt2p unat_p2)
-  finally have \<open>unat (2 :: 'a word) * unat ((2 :: 'a word) ^ n) < 2 ^ LENGTH('a)\<close>
-     .
-  then have [simp]: \<open>unat (2 * (2 :: 'a word) ^ n) = unat (2 :: 'a word) * unat ((2 :: 'a word) ^ n)\<close>
-    using unat_mult_lem[of \<open>2 :: 'a word\<close> \<open>(2 :: 'a word) ^ n\<close>]
-    by auto
-  have [simp]: \<open>(0::nat) < unat ((2::'a word) ^ n)\<close>
-    by (simp add: Suc_lessD le(2) unat_p2)
-
-  show ?case
-    using IH(1)[of m] le(2-)
-    by (auto simp: less_Suc_eq word_less_nat_alt
-      simp del: unat_lt2p)
-qed
-
-lemma pow2_mono_word_le:
-  \<open>m < LENGTH('a) \<Longrightarrow> n < LENGTH('a) \<Longrightarrow> m \<le> n \<Longrightarrow> (2 :: 'a :: len word) ^m  \<le> 2 ^ n\<close>
-  using pow2_mono_word_less[of m n, where 'a = 'a]
-  by (cases \<open>m = n\<close>) auto
-
-lemma unat_le_uint32_max_no_bit_set:
-  fixes n :: \<open>'a::len word\<close>
-  assumes less: \<open>unat n \<le> uint32_max\<close> and
-    n: \<open>n !! na\<close> and
-    32: \<open>32 < LENGTH('a)\<close>
-  shows \<open>na < 32\<close>
-proof (rule ccontr)
-  assume H: \<open>\<not> ?thesis\<close>
-  have na_le: \<open>na < LENGTH('a)\<close>
-    using test_bit_bin[THEN iffD1, OF n]
-    by auto
-  have \<open>(2 :: nat) ^ 32 < (2 :: nat) ^ LENGTH('a)\<close>
-    using 32 power_strict_increasing_iff rel_simps(49) semiring_norm(76) by blast
-  then have [simp]: \<open>(4294967296::nat) mod (2::nat) ^ LENGTH('a) = (4294967296::nat)\<close>
-    by (auto simp:  word_le_nat_alt unat_numeral uint_max_def mod_less
-      simp del: unat_bintrunc)
-  have \<open>(2 :: 'a word) ^ na \<ge> 2 ^ 32\<close>
-    using pow2_mono_word_le[OF 32 na_le] H by auto
-  also have \<open>n \<ge> (2 :: 'a word) ^ na\<close>
-    using assms
-    unfolding uint32_max_def
-    by (auto dest!: bang_is_le)
-  finally have \<open>unat n > uint32_max\<close>
-      supply [[show_sorts]]
-    unfolding word_le_nat_alt
-    by (auto simp:  word_le_nat_alt unat_numeral uint_max_def
-      simp del: unat_bintrunc)
-
-   then show False
-    using less by auto
-qed
-
-lemma le32_enum: \<open>na < (32 :: nat) \<longleftrightarrow> na \<in> {0..<32}\<close>
-  by auto
 
 lemma bin_nth2_32_iff: \<open>bin_nth 4294967295 na \<longleftrightarrow> na < 32\<close>
   by (auto simp: bin_nth_Bit1 bin_nth_Bit0 nat_less_numeral_unfold)
@@ -139,91 +43,9 @@ lemma uint32_of_uint64_uint64_of_uint32[simp]: \<open>uint32_of_uint64 (uint64_o
   by (auto simp: uint64_of_uint32_def uint32_of_uint64_def
     nat_of_uint64_uint64_of_nat_id nat_of_uint32_le_uint32_max nat_of_uint32_le_uint64_max)
 
-lemma uint64_enumerate_all:
-  fixes  n :: uint64
-   assumes \<open>(P 0)\<close> and
-      \<open>(\<And>n. nat_of_uint64 n \<le> 2 ^ 64 \<Longrightarrow> n \<ge> 1 \<Longrightarrow> P (n))\<close>
-    shows \<open>P n\<close>
-    using assms(1) assms(2)[of \<open>n\<close>] nat_of_uint64_le_uint64_max[of n]
-  apply (cases \<open>n = 0\<close>)
-  subgoal
-    by (auto simp: uint64_max_def nat_of_uint64_ge_minus)
-  subgoal
-    apply (subgoal_tac \<open>n \<ge> 1\<close>)
-    apply auto
-    apply (auto simp: uint64_max_def)
-    by (metis nat_geq_1_eq_neqz nat_of_uint64_012(1) nat_of_uint64_012(3) nat_of_uint64_le_iff word_nat_of_uint64_Rep_inject)
-  done
-
-text \<open>This lemma is very trivial but maps an \<^typ>\<open>64 word\<close> to its list counterpart. This
-  especially allows to combine two numbers together via ther bit representation (which should be
-  faster than enumerating all numbers).
-\<close>
-lemma ex_rbl_word64:
-   \<open>\<exists>a64 a63 a62 a61 a60 a59 a58 a57 a56 a55 a54 a53 a52 a51 a50 a49 a48 a47 a46 a45 a44 a43 a42 a41
-     a40 a39 a38 a37 a36 a35 a34 a33 a32 a31 a30 a29 a28 a27 a26 a25 a24 a23 a22 a21 a20 a19 a18 a17
-     a16 a15 a14 a13 a12 a11 a10 a9 a8 a7 a6 a5 a4 a3 a2 a1.
-     to_bl (n :: 64 word) =
-         [a64, a63, a62, a61, a60, a59, a58, a57, a56, a55, a54, a53, a52, a51, a50, a49, a48, a47,
-          a46, a45, a44, a43, a42, a41, a40, a39, a38, a37, a36, a35, a34, a33, a32, a31, a30, a29,
-          a28, a27, a26, a25, a24, a23, a22, a21, a20, a19, a18, a17, a16, a15, a14, a13, a12, a11,
-          a10, a9, a8, a7, a6, a5, a4, a3, a2, a1]\<close> (is ?A) and
-  ex_rbl_word64_le_uint32_max:
-    \<open>unat n \<le> uint32_max \<Longrightarrow> \<exists>a31 a30 a29 a28 a27 a26 a25 a24 a23 a22 a21 a20 a19 a18 a17 a16 a15
-        a14 a13 a12 a11 a10 a9 a8 a7 a6 a5 a4 a3 a2 a1 a32.
-      to_bl (n :: 64 word) =
-      [False, False, False, False, False, False, False, False, False, False, False, False, False,
-       False, False, False, False, False, False, False, False, False, False, False, False, False,
-       False, False, False, False, False, False,
-        a32, a31, a30, a29, a28, a27, a26, a25, a24, a23, a22, a21, a20, a19, a18, a17, a16, a15,
-        a14, a13, a12, a11, a10, a9, a8, a7, a6, a5, a4, a3, a2, a1]\<close> (is \<open>_ \<Longrightarrow> ?B\<close>) and
-  ex_rbl_word64_ge_uint32_max:
-    \<open>n AND (2^32 - 1) = 0 \<Longrightarrow> \<exists>a64 a63 a62 a61 a60 a59 a58 a57 a56 a55 a54 a53 a52 a51 a50 a49 a48
-      a47 a46 a45 a44 a43 a42 a41 a40 a39 a38 a37 a36 a35 a34 a33.
-      to_bl (n :: 64 word) =
-      [a64, a63, a62, a61, a60, a59, a58, a57, a56, a55, a54, a53, a52, a51, a50, a49, a48, a47,
-          a46, a45, a44, a43, a42, a41, a40, a39, a38, a37, a36, a35, a34, a33,
-        False, False, False, False, False, False, False, False, False, False, False, False, False,
-        False, False, False, False, False, False, False, False, False, False, False, False, False,
-        False, False, False, False, False, False]\<close> (is \<open>_ \<Longrightarrow> ?C\<close>)
-proof -
-  have [simp]: "n > 0 \<Longrightarrow> length xs = n \<longleftrightarrow>
-     (\<exists>y ys. xs = y # ys \<and> length ys = n - 1)" for ys n xs
-    by (cases xs) auto
-  show H: ?A
-    using word_bl_Rep'[of n]
-    by (auto simp del: word_bl_Rep')
-
-  show ?B  if \<open>unat n \<le> uint32_max\<close>
-  proof -
-    have H': \<open>m \<ge> 32 \<Longrightarrow> \<not>n !! m\<close> for m
-      using unat_le_uint32_max_no_bit_set[of n m, OF that] by auto
-    show ?thesis using that H'[of 64] H'[of 63] H'[of 62] H'[of 61] H'[of 60] H'[of 59] H'[of 58]
-      H'[of 57] H'[of 56] H'[of 55] H'[of 54] H'[of 53] H'[of 52] H'[of 51] H'[of 50] H'[of 49]
-      H'[of 48] H'[of 47] H'[of 46] H'[of 45] H'[of 44] H'[of 43] H'[of 42] H'[of 41] H'[of 40]
-      H'[of 39] H'[of 38] H'[of 37] H'[of 36] H'[of 35] H'[of 34] H'[of 33] H'[of 32]
-      H'[of 31]
-      using H unfolding unat_def
-      by (clarsimp simp add: test_bit_bl word_size)
-  qed
-  show ?C if \<open>n AND (2^32 - 1) = 0\<close>
-  proof -
-    note H' =  test_bit_bl[of \<open>n AND (2^32 - 1)\<close> m for m, unfolded word_size, simplified]
-    have [simp]: \<open>(n AND 4294967295) !! m = False\<close> for m
-      using that by auto
-    show ?thesis
-      using H H'[of 0]
-      H'[of 32] H'[of 31] H'[of 30] H'[of 29] H'[of 28] H'[of 27] H'[of 26] H'[of 25] H'[of 24]
-      H'[of 23] H'[of 22] H'[of 21] H'[of 20] H'[of 19] H'[of 18] H'[of 17] H'[of 16] H'[of 15]
-      H'[of 14] H'[of 13] H'[of 12] H'[of 11] H'[of 10] H'[of 9] H'[of 8] H'[of 7] H'[of 6]
-      H'[of 5] H'[of 4] H'[of 3] H'[of 2] H'[of 1]
-      unfolding unat_def word_size that
-      by (clarsimp simp add: word_size bl_word_and word_add_rbl)
-  qed
-qed
-
 lemma take_only_lower32_le_uint32_max_ge_uint32_max:
-  \<open>nat_of_uint64 n \<le> uint32_max \<Longrightarrow> nat_of_uint64 m \<ge> uint32_max \<Longrightarrow> take_only_lower32 m = 0 \<Longrightarrow> take_only_lower32 (n + m) = n\<close>
+  \<open>nat_of_uint64 n \<le> uint32_max \<Longrightarrow> nat_of_uint64 m \<ge> uint32_max \<Longrightarrow> take_only_lower32 m = 0 \<Longrightarrow>
+    take_only_lower32 (n + m) = n\<close>
   unfolding take_only_lower32_def
   apply transfer
   subgoal for m n
@@ -322,17 +144,6 @@ lemma watcher_enc_extract_bool_False:
     nat_of_uint32_le_uint32_max nat_of_uint64_1_32 take_only_lower32_1_32 AND_2_32_bool
       take_only_lower32_le_uint32_max_ge_uint32_max le_uint32_max_AND2_32_eq0)
 
-lemma numeral_uint64_eq_iff[simp]:
- \<open>numeral m \<le> (2^64-1 :: nat) \<Longrightarrow> numeral n \<le> (2^64-1 :: nat) \<Longrightarrow> ((numeral m :: uint64) = numeral n) \<longleftrightarrow> numeral m = (numeral n :: nat)\<close>
-  by (subst word_nat_of_uint64_Rep_inject[symmetric])
-    (auto simp: uint64_max_def)
-
-
-lemma numeral_uint64_eq0_iff[simp]:
- \<open>numeral n \<le> (2^64-1 :: nat) \<Longrightarrow> ((0 :: uint64) = numeral n) \<longleftrightarrow> 0 = (numeral n :: nat)\<close>
-  by (subst word_nat_of_uint64_Rep_inject[symmetric])
-    (auto simp: uint64_max_def)
-
 
 lemma watcher_enc_extract_bool:
   assumes \<open>(n, (L, b)) \<in> watcher_enc \<close>
@@ -378,17 +189,6 @@ definition to_watcher_code :: \<open>nat \<Rightarrow> uint32 \<Rightarrow> bool
   [code del]:
     \<open>to_watcher_code = (\<lambda>a L b. (a, uint64_of_uint32 L OR (if b then 1 << 32 else (0 :: uint64))))\<close>
 
-lemma transfer_pow_uint64: \<open>Transfer.Rel (rel_fun cr_uint64 (rel_fun (=) cr_uint64)) (^) (^)\<close>
-  apply (auto simp: Transfer.Rel_def rel_fun_def cr_uint64_def)
-  subgoal for x y
-    by (induction y)
-      (auto simp: one_uint64.rep_eq times_uint64.rep_eq)
-  done
-
-lemma shiftl_t2n_uint64: \<open>n << m = n * 2 ^ m\<close> for n :: uint64
-  apply transfer
-  prefer 2 apply (rule transfer_pow_uint64)
-  by (auto simp: shiftl_t2n)
 
 lemma to_watcher_code[code]:
   \<open>to_watcher_code a L b = (a, uint64_of_uint32 L OR (if b then 4294967296 else (0 :: uint64)))\<close>
